src/Init/Data/Iterators/Lemmas.lean
@@ -9,3 +9,4 @@ prelude
 public import Init.Data.Iterators.Lemmas.Consumers
 public import Init.Data.Iterators.Lemmas.Combinators
 public import Init.Data.Iterators.Lemmas.Producers
+public import Init.Data.Iterators.Lemmas.Transport
